tmp

theories/Strl.v
@@ -58,3 +58,68 @@ Proof.
 Defined.
 Definition slsplice sl i sl2 :=
   slcat (slcat (slsub sl 0 i) sl2) (slsub sl (i + sllength sl2) (sllength sl)).
+Definition list_of_strl (sl: strl) := List.concat (map to_list (proj1_sig sl)).
+Notation "'LO'" := list_of_strl.
+Definition slequiv sl1 sl2 := list_of_strl sl1 = list_of_strl sl2.
+Infix "~" := slequiv (at level 10).
+Lemma list_get:
+  forall sl i, slget sl i = nth (to_nat i) (LO sl) 0.
+Proof.
+  intros. destruct sl. unfold slget, list_of_strl. simpl. clear f.
+  generalize i. induction x; intro.
+    simpl. now destruct (_:nat).
+    simpl. destruct ltb eqn:LT.
+      rewrite app_nth1. apply get_spec.
+      rewrite <-length_spec. lia.
+    rewrite IHx. rewrite app_nth2, <-length_spec. f_equal. lia.
+    rewrite <-length_spec. lia.
+Qed.
+Lemma list_cat:
+  forall sl1 sl2, LO (slcat sl1 sl2) = LO sl1 ++ LO sl2.
+Proof.
+  intros. destruct sl1, sl2. unfold slcat, list_of_strl. simpl.
+  now rewrite map_app, concat_app.
+Qed.
+Lemma list_sub:
+  forall sl i n, LO (slsub sl i n) = firstn (to_nat n) (skipn (to_nat i) (LO sl)).
+Proof.
+  intros. destruct sl. unfold slsub, list_of_strl. simpl. clear f.
+  generalize i n. induction x; intros; simpl.
+    destruct eqb; now rewrite skipn_nil, firstn_nil.
+    destruct eqb eqn:EQ.
+      apply eqb_correct in EQ. now rewrite EQ.
+      destruct ltb eqn:LT.
+      - simpl. rewrite IHx, skipn_app, firstn_app.
+        f_equal. apply sub_spec.
+        f_equal. rewrite length_spec_int, sub_spec, length_firstn, length_skipn. lia.
+        f_equal. rewrite <-length_spec. lia.
+      - rewrite IHx, skipn_app.
+        f_equal. rewrite (skipn_all2 (to_list a)), app_nil_l.
+        f_equal. rewrite <-length_spec. lia.
+        rewrite <-length_spec. lia.
+Qed.
+Lemma fold_add:
+  forall l n, fold_left add l n = fold_left add l 0 + n.
+Proof.
+  induction l. simpl. lia. simpl. intro. rewrite IHl, (IHl (0+a)). lia.
+Qed.
+Lemma list_length:
+  forall sl, sllength sl = of_nat (List.length (LO sl)).
+Proof.
+  intros. destruct sl. unfold sllength, list_of_strl. simpl. clear f.
+  induction x. easy.
+  unfold _sllength in *. simpl. rewrite fold_add.
+  rewrite IHx. rewrite length_app. rewrite <-length_spec. lia.
+Qed.
+Lemma list_splice:
+  forall sl1 i sl2, LO (slsplice sl1 i sl2) =
+    firstn (to_nat i) (LO sl1)++LO sl2++skipn (to_nat (i + sllength sl2)) (LO sl1).
+Proof.
+  intros. destruct sl1, sl2. unfold slsplice, sllength, slsub, list_of_strl. simpl. clear f f0.
+  
+
+Lemma equiv_get:
+  forall sl1 sl2 i, sl1 ~ sl2 -> slget sl1 i = slget sl2 i.
+Proof.
+  intros. now rewrite !list_get, H.
+Qed.
